spec/abstract/Structures_A.thy
@@ -373,6 +373,7 @@ datatype thread_state
   = Running
   | Inactive
   | Restart
+  | YieldTo
   | BlockedOnReceive obj_ref "obj_ref option"
   | BlockedOnSend obj_ref sender_payload
   | BlockedOnReply
@@ -386,12 +387,14 @@ record tcb =
  tcb_vtable        :: cap
  tcb_ipcframe      :: cap
  tcb_fault_handler :: cap
+ tcb_timeout_handler :: cap
  tcb_state         :: thread_state
  tcb_ipc_buffer    :: vspace_ref
  tcb_fault         :: "fault option"
  tcb_bound_notification     :: "obj_ref option"
  tcb_mcpriority    :: priority
  tcb_sched_context :: "obj_ref option"
+ tcb_yield_to      :: "obj_ref option"
  tcb_reply         :: "obj_ref option"
  tcb_arch          :: arch_tcb
 
@@ -402,6 +405,7 @@ where
   "runnable (Running)               = True"
 | "runnable (Inactive)              = False"
 | "runnable (Restart)               = True"
+| "runnable (YieldTo)               = True"
 | "runnable (BlockedOnReceive _ _)  = False"
 | "runnable (BlockedOnSend x y)     = False"
 | "runnable (BlockedOnNotification x) = False"
@@ -415,12 +419,14 @@ definition
       tcb_vtable   = NullCap,
       tcb_ipcframe = NullCap,
       tcb_fault_handler = NullCap,
+      tcb_timeout_handler = NullCap,
       tcb_state    = Inactive,
       tcb_ipc_buffer = 0,
       tcb_fault      = None,
       tcb_bound_notification  = None,
       tcb_mcpriority = minBound,
       tcb_sched_context = None,
+      tcb_yield_to   = None,
       tcb_reply      = None,
       tcb_arch       = default_arch_tcb\<rparr>"
 
@@ -433,10 +439,13 @@ record refill =
 
 record sched_context =
   sc_period     :: ticks
+  sc_consumed   :: ticks
   sc_tcb        :: "obj_ref option"
   sc_ntfn       :: "obj_ref option"
   sc_refills    :: "refill list"
   sc_refill_max :: nat
+  sc_badge      :: badge
+  sc_yield_from :: "obj_ref option"
   sc_replies    :: "obj_ref list"
 
 definition "MIN_REFILLS = 2"
@@ -446,10 +455,13 @@ definition
   default_sched_context :: sched_context where
   "default_sched_context \<equiv> \<lparr>
     sc_period     = 0,
+    sc_consumed     = 0,
     sc_tcb        = None,
     sc_ntfn       = None,
     sc_refills    = [\<lparr>r_time=0, r_amount=0\<rparr>],
     sc_refill_max = 0,
+    sc_badge      = 0,
+    sc_yield_from = None,
     sc_replies    = []
   \<rparr>"
 
@@ -618,7 +630,7 @@ capability slots within a TCB.
 *}
 definition
   tcb_cnode_index :: "nat \<Rightarrow> cnode_index" where
-  "tcb_cnode_index n \<equiv> to_bl (of_nat n :: 2 word)"
+  "tcb_cnode_index n \<equiv> to_bl (of_nat n :: 3 word)"
 
 text {* Zombie capabilities store the bit size of the CNode cap they were
 created from or None if they were created from a TCB cap. This function
@@ -689,7 +701,8 @@ definition tcb_cnode_map :: "tcb \<Rightarrow> cnode_index \<Rightarrow> cap opt
    [tcb_cnode_index 0 \<mapsto> tcb_ctable tcb,
     tcb_cnode_index 1 \<mapsto> tcb_vtable tcb,
     tcb_cnode_index 2 \<mapsto> tcb_ipcframe tcb,
-    tcb_cnode_index 3 \<mapsto> tcb_fault_handler tcb]"
+    tcb_cnode_index 3 \<mapsto> tcb_fault_handler tcb,
+    tcb_cnode_index 4 \<mapsto> tcb_timeout_handler tcb]"
 
 definition cap_of :: "kernel_object \<Rightarrow> cnode_index \<Rightarrow> cap option"
   where
