spec/abstract/ARM/ArchFault_A.thy
@@ -24,7 +24,7 @@ fun make_arch_fault_msg :: "arch_fault \<Rightarrow> obj_ref \<Rightarrow> (data
 where
  "make_arch_fault_msg (VMFault vptr archData) thread = do
      pc \<leftarrow> as_user thread getRestartPC;
-     return (5, pc # vptr # archData) od"
+     return (6, pc # vptr # archData) od"
 
 definition
   handle_arch_fault_reply :: "arch_fault \<Rightarrow> obj_ref \<Rightarrow> data \<Rightarrow> data list \<Rightarrow> (bool,'z::state_ext) s_monad"
