spec/abstract/ARM/Arch_A.thy
@@ -15,7 +15,7 @@ Entry point for architecture dependent definitions.
 chapter "Toplevel ARM Definitions"
 
 theory Arch_A
-imports "../TcbAcc_A"
+imports "../CSpace_A"
 begin
 
 context Arch begin global_naming ARM_A
