spec/abstract/IpcCancel_A.thy
@@ -135,6 +135,14 @@ where
     when (hd replies = r) $ sched_context_donate sc_ptr caller
   od"
 
+definition
+  unbind_from_reply :: "obj_ref \<Rightarrow> (unit, det_ext) s_monad"
+where
+  "unbind_from_reply tptr \<equiv> do
+    reply_opt \<leftarrow> thread_get tcb_reply tptr;
+    maybeM reply_remove reply_opt
+  od"
+
 text {* Push a reply object to the call stack. *}
 definition
   reply_push :: "obj_ref \<Rightarrow> obj_ref \<Rightarrow> obj_ref \<Rightarrow> bool \<Rightarrow> unit det_ext_monad"
@@ -257,34 +265,26 @@ definition
    od"
 
 definition
-  possible_switch_to :: "obj_ref \<Rightarrow> bool \<Rightarrow> unit det_ext_monad" where
-  "possible_switch_to target on_same_prio \<equiv> do
+  possible_switch_to :: "obj_ref \<Rightarrow> unit det_ext_monad" where
+  "possible_switch_to target \<equiv> do
      sc_opt \<leftarrow> thread_get tcb_sched_context target;
      inq \<leftarrow> gets $ in_release_queue target;
      when (sc_opt \<noteq> None \<and> \<not>inq) $ do
-       cur \<leftarrow> gets cur_thread;
-       cur_dom \<leftarrow> gets cur_domain;
-       cur_prio \<leftarrow> ethread_get tcb_priority cur;
-       target_dom \<leftarrow> ethread_get tcb_domain target;
-       target_prio \<leftarrow> ethread_get tcb_priority target;
-       action \<leftarrow> gets scheduler_action;
-       if (target_dom \<noteq> cur_dom) then tcb_sched_action tcb_sched_enqueue target
-       else do
-         if (target_prio > cur_prio \<or> (target_prio = cur_prio \<and> on_same_prio))
-                \<and> action = resume_cur_thread then set_scheduler_action $ switch_thread target
-           else tcb_sched_action tcb_sched_enqueue target;
-         case action of switch_thread _ \<Rightarrow> reschedule_required | _ \<Rightarrow> return ()
+     cur_dom \<leftarrow> gets cur_domain;
+     target_dom \<leftarrow> ethread_get tcb_domain target;
+     action \<leftarrow> gets scheduler_action;
+
+     if (target_dom \<noteq> cur_dom) then
+       tcb_sched_action tcb_sched_enqueue target
+     else if (action \<noteq> resume_cur_thread) then
+       do
+         reschedule_required;
+         tcb_sched_action tcb_sched_enqueue target
        od
-     od
+     else
+       set_scheduler_action $ switch_thread target
+   od
    od"
-
-definition
-  attempt_switch_to :: "obj_ref \<Rightarrow> unit det_ext_monad" where
-  "attempt_switch_to target \<equiv> possible_switch_to target True"
-
-definition
-  switch_if_required_to :: "obj_ref \<Rightarrow> unit det_ext_monad" where
-  "switch_if_required_to target \<equiv> possible_switch_to target False"
 
 text {* Cancel all message operations on threads currently queued within this
 synchronous message endpoint. Threads so queued are placed in the Restart state.
@@ -327,7 +327,7 @@ where
                 st \<leftarrow> get_thread_state t;
                 if blocking_ipc_badge st = badge then do
                   set_thread_state t Restart;
-                  switch_if_required_to t;
+                  possible_switch_to t;
                   return False
                 od
                 else return True
@@ -403,7 +403,7 @@ where
      case ntfn_obj ntfn of WaitingNtfn queue \<Rightarrow> do
                       _ \<leftarrow> set_notification ntfnptr $ ntfn_set_obj ntfn IdleNtfn;
                       mapM_x (\<lambda>t. do set_thread_state t Restart;
-                                     switch_if_required_to t od) queue;
+                                     possible_switch_to t od) queue;
                       do_extended_op (reschedule_required)
                      od
                | _ \<Rightarrow> return ()
@@ -441,31 +441,6 @@ where
     sc \<leftarrow> get_sched_context sc_ptr;
     when (sc_tcb sc \<noteq> None) $ sched_context_unbind_tcb sc_ptr
   od"
-
-text {* Finalise a capability if the capability is known to be of the kind
-which can be finalised immediately. This is a simplified version of the
-@{text finalise_cap} operation. *}
-fun
-  fast_finalise :: "cap \<Rightarrow> bool \<Rightarrow> unit det_ext_monad"
-where
-  "fast_finalise NullCap                 final = return ()"
-| "fast_finalise (ReplyCap r)            final =
-      (when final $ reply_remove r)"
-| "fast_finalise (EndpointCap r b R)     final =
-      (when final $ cancel_all_ipc r)"
-| "fast_finalise (NotificationCap r b R) final =
-      (when final $ do
-          sched_context_maybe_unbind_ntfn r;
-          unbind_maybe_notification r;
-          cancel_all_signals r
-       od)"
-| "fast_finalise (SchedContextCap sc b)    final =
-      (when final $ do
-          sched_context_unbind_all_tcbs sc;
-          sched_context_unbind_ntfn sc;
-          sched_context_clear_replies sc
-      od)"
-| "fast_finalise _ _ = fail"
 
 text {* The optional IRQ stored in a capability, presented either as an optional
 value or a set. *}
@@ -567,19 +542,6 @@ where
       od
   od"
 
-text {* Delete a capability with the assumption that the fast finalisation
-process will be sufficient. *}
-definition
-  cap_delete_one :: "cslot_ptr \<Rightarrow> unit det_ext_monad" where
- "cap_delete_one slot \<equiv> do
-    cap \<leftarrow> get_cap slot;
-    unless (cap = NullCap) $ do
-      final \<leftarrow> is_final_cap cap;
-      fast_finalise cap final;
-      empty_slot slot NullCap
-    od
-  od"
-
 text {* Cancel the message receive operation of a thread waiting for a Reply
 capability it has issued to be invoked. *}
 definition
@@ -620,17 +582,6 @@ where
         | BlockedOnNotification event \<Rightarrow> cancel_signal tptr event
         | BlockedOnReply \<Rightarrow> reply_cancel_ipc tptr
         | _ \<Rightarrow> return ()
-   od"
-
-text {* Suspend a thread, cancelling any pending operations and preventing it
-from further execution by setting it to the Inactive state. *}
-definition
-  suspend :: "obj_ref \<Rightarrow> unit det_ext_monad"
-where
-  "suspend thread \<equiv> do
-     cancel_ipc thread;
-     set_thread_state thread Inactive;
-     do_extended_op (tcb_sched_action (tcb_sched_dequeue) thread)
    od"
 
 end
